{
 "cells": [
  {
   "cell_type": "markdown",
   "metadata": {},
   "source": [
    "## Section 1.5 - Circles"
   ]
  },
  {
   "cell_type": "markdown",
   "metadata": {},
   "source": [
    "#### 1. Find an equation of the line containing the centers of the two circles\n",
    "\n",
    "$ x^2 + y^2 -4x +6y + 4 = 0 \\text { and } \\\\\n",
    "x^2 + y^2 + 6x + 4y + 9 = 0 .\n",
    "$"
   ]
  },
  {
   "cell_type": "markdown",
   "metadata": {},
   "source": [
    "Solution:\n",
    "\n",
    "Let's first express the equations in the following form:\n",
    "\n",
    "$(x-h)^2 + (y-k)^2 = r^2$\n",
    "\n",
    "$\n",
    "x^2 + y^2 - 4x + 6y + 4 = 0   \\\\\n",
    "\\implies (x^2 - 4x + 4) + (y^2 + 6y + 9) - 9 = 0   \\\\\n",
    "\\implies (x - 2)^2 + (y + 3)^2 = 3^2  \\\\\n",
    "$\n",
    "\n",
    "Radius of the circle is $(2,-3)$ and radius $3$.\n",
    "\n",
    "$\n",
    "x^2 + y^2 + 6x + 4y + 4 = 0   \\\\\n",
    "\\implies (x^2 + 6x + 9) + (y^2 + 4y + 4) - 9 = 0   \\\\\n",
    "\\implies (x + 3)^2 + (y + 2)^2 = 3^2  \\\\\n",
    "$\n",
    "\n",
    "Radius of the circle is $(-3,-2)$ and radius $3$.\n",
    "\n",
    "Let's find the straight line joining that contains the centers $(2,-3), (-3,-2)$.\n",
    "\n",
    "$\n",
    "\\dfrac{(y - (-3))}{(-3-(-2))} = \\dfrac{(x-2)}{(2-(-3))}  \\\\\n",
    "\\implies \\dfrac{y+3}{-1} = \\dfrac{x-2}{5} \\\\\n",
    "\\implies 5y + 15 = -x + 2  \\\\\n",
    "\\implies x + 5y + 13 = 0\n",
    "$"
   ]
  },
  {
   "cell_type": "markdown",
   "metadata": {},
   "source": [
    "#### 2. The line $x-2y+4=0$ is tangent to a circle at $(0,2)$. The line $y=2x-7$ is tangent to the same circle $(3,-1)$. Find the center of the circle."
   ]
  },
  {
   "cell_type": "markdown",
   "metadata": {},
   "source": [
    "Solution:\n",
    "    \n",
    "We know that the tangents to a circle are perpendicular to the lines connecting the center of the circle and the points of tangency.\n",
    "\n",
    "Let's find the equations of the lines that connect the center of the circle and the points of tangency.\n",
    "\n",
    "Slope of the line $(1)$: $x - 2y + 4 = 0$ is $\\dfrac{1}{2}$  \n",
    "Slope of the line perpendicular to the above line is $-2$.\n",
    "Hence the equation of the line with slope $-2$ and passing through $(0,2)$ can be written as:\n",
    "\n",
    "$\n",
    "\\dfrac{y-2}{x-0} = 2  \\\\\n",
    "2x - y + 2 = 0 \\cdots (3)\n",
    "$\n",
    "\n",
    "\n",
    "Slope of the line $(2)$: $y = 2x - 7$ is $2$  \n",
    "Slope of the line perpendicular to the above line is $-\\dfrac{1}{2}$.\n",
    "Hence the equation of the line with slope $-\\dfrac{1}{2}$ and passing through $(3,-1)$ can be written as:\n",
    "\n",
    "\n",
    "$\n",
    "\\dfrac{y+1}{x-3} = -\\dfrac{1}{2}  \\\\\n",
    "2y + 2 = -x + 3   \\\\\n",
    "x + 2y -1 = 0 \\cdots (4)\n",
    "$\n",
    "\n",
    "Now, the solution of the equations (3) and (4), is the co-ordinate of the center of the circle.\n",
    "\n",
    "$\n",
    "2x - y + 2 = 0 \\cdots (3)  \\\\\n",
    "\\implies x = \\dfrac{y-2}{2}  \\\\\n",
    "$\n",
    "\n",
    "$\n",
    "x + 2y -1 = 0 \\cdots (4) \\\\\n",
    "\\implies x = -2y + 1 \\\\\n",
    "$\n",
    "\n",
    "$\n",
    "\\dfrac{y-2}{2} = -2y + 1 \\\\\n",
    "\\implies y = \\dfrac{4}{5}\n",
    "$\n",
    "\n",
    "From (4), we get,\n",
    "\n",
    "$\n",
    "x = (-2)\\dfrac{4}{5} + 1 = -\\dfrac{3}{5}\n",
    "$\n",
    "\n",
    "The center of the circle is at $\\bigg(-\\dfrac{3}{5},\\dfrac{4}{5}\\bigg)$."
   ]
  },
  {
   "cell_type": "markdown",
   "metadata": {},
   "source": [
    "#### 3. If the equation of the circle is $x^2 + y^2 = r^2$ and the equation of the tangent line is $y = mx + b$, show that:\n",
    "$\n",
    "(a) \\ r^2(1+m^2) = b^2  \\\\\n",
    "(b) \\text{ The point of tangency is} \\bigg(-\\dfrac{r^2m}{b}, \\dfrac{r^2}{b}\\bigg)  \\\\\n",
    "(c) \\text{ The tangent line is perpendicular to the line containing the center of the circle and the point of tangency.}\n",
    "$\n"
   ]
  },
  {
   "cell_type": "markdown",
   "metadata": {},
   "source": [
    "Solution:\n",
    "\n",
    "(a) Let's consider that the point of tangency is $(x_1, y_1)$.\n",
    "\n",
    "We can write,\n",
    "\n",
    "$x_1^2 + y_1^2 = r^2 \\qquad (1) \\\\ $ \n",
    "$y_1 = mx_1 + b \\qquad (2) $\n",
    "\n",
    "By substituting $y_1$ in $(1)$, we get,\n",
    "\n",
    "$\n",
    "x_1^2 + (mx_1 + b)^2 = r^2  \\\\ \n",
    "x_1^2 + (m^2x_1^2 + 2mbx_1 + b^2) = r^2 \\\\\n",
    "(1+m^2)x_1^2 + 2mbx_1 + (b^2 - r^2) = 0 \\qquad (3) \\\\\n",
    "$ \n",
    "\n",
    "Now, roots of an quadratic equation can be expressed as:\n",
    "$\n",
    "ax^2 + bx + c = 0  \\\\\n",
    "x = \\dfrac{-b \\pm \\sqrt{b^2-4ac}}{2a}\n",
    "$\n",
    "\n",
    "When the two roots are equal, we can write,\n",
    "\n",
    "$\n",
    "\\dfrac{-b + \\sqrt{b^2-4ac}}{2a} = \\dfrac{-b - \\sqrt{b^2-4ac}}{2a}  \\\\\n",
    "\\implies \\sqrt{b^2-4ac} = 0 \\\\\n",
    "\\implies b^2 = 4ac \\qquad (4)\n",
    "$\n",
    "\n",
    "Since, the equations $(1)$ and $(2)$ have only solution, we can write from $(3)$ and $(4)$,\n",
    "\n",
    "$\n",
    "(2mb)^2 - 4(1+m^2)(b^2 - r^2) = 0    \\\\\n",
    "\\implies 4m^2b^2 - 4b^2 - 4m^2b^2 + 4r^2 + 4m^2r^2 = 0    \\\\\n",
    "\\implies r^2(1+m^2) = b^2  \\qquad(5)\n",
    "$\n",
    "\n",
    "(b) From above, we can write,\n",
    "\n",
    "$\n",
    "x_1 = -\\dfrac{2mb}{2(1+m^2)} = -\\dfrac{mb}{b^2/r^2} = -\\dfrac{r^2m}{b}\n",
    "$\n",
    "\n",
    "From $(2)$,\n",
    "\n",
    "$\n",
    "y_1 = m\\bigg( -\\dfrac{r^2m}{b} \\bigg) + b \\\\\n",
    "\\implies y_1 = \\dfrac{1}{b}(-r^2m^2 + b^2)\n",
    "$\n",
    "\n",
    "From $(5)$,\n",
    "\n",
    "$\n",
    "r^2 = -r^2m^2 + b^2 \\\\\n",
    "y_1 = \\dfrac{r^2}{b}\n",
    "$\n",
    "\n",
    "Hence, the point of tangency $ =  \\bigg(-\\dfrac{r^2m}{b}, \\dfrac{r^2}{b}\\bigg)$\n",
    "\n",
    "(c) The equation of the circle $x^2 + y^2 = r^2$ tells us that the center is at $(0,0)$.\n",
    "\n",
    "Therefore, the slope of the line connecting $(0,0)$ and $\\bigg(-\\dfrac{r^2m}{b}, \\dfrac{r^2}{b}\\bigg)$ can be writtes as:\n",
    "\n",
    "$\n",
    "m_1 = \\dfrac{\\dfrac{r^2}{b}-0}{-\\dfrac{r^2m}{b}-0} = -\\dfrac{1}{m}\n",
    "$\n",
    "\n",
    "Slope of the tangent $y = xm + b$ is $m_2 = m.$\n",
    "\n",
    "$\\therefore m_1m_2 = -1$, which proves that the tangent line is perpendicular to the line containing the center of the circle and the point of tangency."
   ]
  },
  {
   "cell_type": "markdown",
   "metadata": {},
   "source": [
    "#### 4. Find the equation of the circle with endpoints of a diameter at $(1,4)$ and $(-3,2)$.\n",
    "\n",
    "Solution: \n",
    "\n",
    "The center of the circle is located at the midpoint of $(1,4)$ and $(-3,2)$ = $\\bigg(\\dfrac{1-3}{2}, \\dfrac{4+2}{2}\\bigg) = (-1,3)$\n",
    "We can also calculate the radius by finding the distance between $(1,4)$ and $(-3,2)$.\n",
    "\n",
    "$r = \\dfrac{1}{2} \\times \\sqrt{(1+3)^2 + (4-2)^2} = \\dfrac{1}{2} \\cdot 2\\sqrt5 = \\sqrt5$\n",
    "\n",
    "The standard equation of the circle can be written as:\n",
    "\n",
    "$\n",
    "(x+1)^2 + (y-3)^2 = (\\sqrt5)^2    \\\\\n",
    "\\therefore (x+1)^2 + (y-3)^2 = 5   \\\\\n",
    "x^2 + 2x + 1 + y^2 - 6y + 9 = 5 \\\\\n",
    "\\therefore x^2 + y^2 + 2x - 6y + 5 = 0 \\\\\n",
    "$"
   ]
  }
 ],
 "metadata": {
  "kernelspec": {
   "display_name": "Python 3",
   "language": "python",
   "name": "python3"
  },
  "language_info": {
   "codemirror_mode": {
    "name": "ipython",
    "version": 3
   },
   "file_extension": ".py",
   "mimetype": "text/x-python",
   "name": "python",
   "nbconvert_exporter": "python",
   "pygments_lexer": "ipython3",
   "version": "3.7.9"
  }
 },
 "nbformat": 4,
 "nbformat_minor": 4
}
